proof-checker/fullProgScript.sml
@@ -1,0 +1,81 @@
+open preamble ml_progLib ml_translatorLib
+open proofCheckerProgTheory
+open ml_translatorTheory ml_translatorLib
+open proofCheckerTheory astPP2
+
+val _ = new_theory "fullProg";
+
+val _ = translation_extends "proofCheckerProg";
+
+(*
+local
+  val ths = ml_translatorLib.eq_lemmas();
+in
+  fun find_equality_type_thm tm =
+    first (can (C match_term tm) o rand o snd o strip_imp o concl) ths
+end
+
+val EqualityType_PROOFCHECKER_VARS_TYPE = find_equality_type_thm``PROOFCHECKER_VARS_TYPE``;
+val EqualityType_WORD = find_equality_type_thm``WORD``;
+
+val EqualityType_PROOFCHECKER_TRM_TYPE
+
+val PROOFCHECKER_TRM_TYPE_no_closures = Q.prove(
+  `∀a b c.
+  EqualityType a ⇒
+  PROOFCHECKER_TRM_TYPE a b c ⇒ no_closures c`,
+  ho_match_mp_tac PROOFCHECKER_TRM_TYPE_ind \\
+  rw[PROOFCHECKER_TRM_TYPE_def] \\
+  rw[no_closures_def] \\
+    TRY (
+    qmatch_assum_rename_tac`LIST_TYPE _ x y` \\
+    qhdtm_x_assum`LIST_TYPE`mp_tac \\
+    last_x_assum mp_tac \\
+    map_every qid_spec_tac[`y`,`x`] \\
+    Induct \\ rw[LIST_TYPE_def] \\
+    rw[no_closures_def] \\
+    metis_tac[] ) \\
+  fs[EqualityType_def] \\ TRY (metis_tac[])>>
+  metis_tac[EqualityType_def,EqualityType_PROOFCHECKER_VARS_TYPE,EqualityType_WORD]);
+
+val ctor_same_type_def = semanticPrimitivesTheory.ctor_same_type_def;
+
+*)
+
+val fu_inst_def = Define`
+  fu_inst = fin_univ varls varls`
+
+val fu_inst_def = Define`
+  fu_inst = fin_univ varls varls`
+
+val ids_loc_inst_def = Define`
+  ids_loc_inst =
+  ids_loc
+  i1 i2 i3 (\x. x = i1)
+  i1 i2 i3
+  i1 i2 i3 i4`
+
+val pt_result_full_def = Define`
+  pt_result_full pt = pt_result fu_inst ids_loc_inst pt`
+
+val res = translate fu_inst_def;
+val res = translate ids_loc_inst_def;
+val res = translate pt_result_full_def;
+
+val ML_code_prog =
+  get_ml_prog_state ()
+  |> clean_state |> remove_snocs
+  |> get_thm
+
+val prog = ML_code_prog |> concl |> strip_comb |> #2 |> el 3
+
+val _ = enable_astPP()
+
+val _ = trace("pp_avoids_symbol_merges",0)
+
+val t = TextIO.openOut("pt_result.sml")
+val _ = TextIO.output(t,term_to_string prog)
+val _ = TextIO.closeOut(t)
+
+
+val _ = export_theory();
